interp/src/prheap.mli
@@ -27,6 +27,7 @@ val prliteral : JsSyntax.literal -> string
 val prprim : JsSyntax.prim -> string
 val prvalue : JsSyntax.value -> string
 val prref : JsSyntax.ref -> string
+val prresvalue : JsSyntax.resvalue -> string
 
 val prdescriptor : JsSyntax.descriptor -> string
 val prfull_descriptor : JsSyntax.full_descriptor -> string
